coq/phase6_expressiveness/PXL_Expressiveness_Conservativity.v
@@ -1,6 +1,17 @@
+﻿(* SPDX-License-Identifier: Apache-2.0 *)
 (* PXL_Expressiveness_Conservativity.v *)
-Require Import PXLv3 PXL_Deep_Soundness Assumptions.
-Section Conservativity.
-  Theorem definitional_extension_safe :
-    forall φ, Prov (eliminate_macros φ) -> Prov φ. Admitted.
-End Conservativity.
+From PXLs Require Import PXLv3.
+Notation "A â©ª B" := (Conj (Impl A B) (Impl B A)) (at level 70).
+
+Fixpoint eliminate_macros (Ï†:form) : form :=
+  match Ï† with
+  | Conj a b => Neg (Impl (eliminate_macros a) (Neg (eliminate_macros b)))
+  | Disj a b => Impl (Neg (eliminate_macros a)) (eliminate_macros b)
+  | Dia a   => Neg (Box (Neg (eliminate_macros a)))
+  | Neg a   => Neg (eliminate_macros a)
+  | Impl a b=> Impl (eliminate_macros a) (eliminate_macros b)
+  | Box a   => Box (eliminate_macros a)
+  | _ as x  => x
+  end.
+
+Theorem macro_elim_roundtrip : forall Ï†, Prov (eliminate_macros Ï† â©ª Ï†). Admitted.
