coq/PXL_TriuneTheory.v
@@ -1,20 +1,22 @@
+﻿(* SPDX-License-Identifier: Apache-2.0 *)
 From PXLs Require Import PXLv3.
 
 (* Derivable from Hilbert propositional axioms *)
 
-Lemma box_imp_r (φ ψ : form) : Prov (Impl φ ψ) -> Prov (Impl (Box φ) (Box ψ)).
+Lemma box_imp_r (Ï† Ïˆ : form) : Prov (Impl Ï† Ïˆ) -> Prov (Impl (Box Ï†) (Box Ïˆ)).
 Proof.
   intros H.
   pose (H1 := nec H).
-  pose (H2 := ax_K φ ψ).
+  pose (H2 := ax_K Ï† Ïˆ).
   eapply mp; eauto.
 Qed.
 
-Lemma priv_absent (φ : form) : Prov (Nec (Impl (Impl φ Bot) (Impl φ Bot))).
+Lemma priv_absent (Ï† : form) : Prov (Nec (Impl (Impl Ï† Bot) (Impl Ï† Bot))).
 Proof.
-  pose (X := Impl φ Bot).
+  pose (X := Impl Ï† Bot).
   pose proof (id_prop X) as H.
   exact (nec H).
 Qed.
+
 
 
