coq/S5_Kripke.v
@@ -1,3 +1,4 @@
+﻿(* SPDX-License-Identifier: Apache-2.0 *)
 From Coq Require Import Logic.Classical.
 
 (*
@@ -130,3 +131,4 @@ Proof.
 Qed.
 
 End S5_Semantics.
+
